CertiGC/gc_spec.v
@@ -164,7 +164,7 @@ Definition forward_spec :=
     PROP (readable_share rsh; writable_share sh;
           super_compatible (g, t_info, roots) f_info outlier;
           forward_p_compatible forward_p roots g;
-          forward_condition g t_info from to; to <> O)
+          forward_condition g t_info from to; to <> O; 0 <= depth <= Int.max_signed)
     LOCAL (temp _from_start (gen_start g from);
            temp _from_limit
                 (offset_val (WORD_SIZE * gen_size t_info from)
