CertiGC/verif_forward.v
@@ -82,85 +82,85 @@ Proof.
   unfold forward_p_address. destruct forward_p.
   - unfold thread_info_rep. Intros.
     assert (Zlength roots = Zlength (live_roots_indices f_info)). {
-      rewrite <- (Zlength_map _ _ (flip Znth (ti_args t_info))), <- H3, Zlength_map.
+      rewrite <- (Zlength_map _ _ (flip Znth (ti_args t_info))), <- H4, Zlength_map.
       reflexivity. }
-    pose proof (Znth_map _ (root2val g) _ H0). hnf in H0. rewrite H10 in H0.
-    rewrite H3, Znth_map in H11 by assumption. unfold flip in H11.
-    remember (Znth z roots) as root. rewrite <- H10 in H0. pose proof (Znth_In _ _ H0).
-    rewrite <- Heqroot in H12. rewrite H10 in H0. unfold Inhabitant_val in H11.
+    pose proof (Znth_map _ (root2val g) _ H0). hnf in H0. rewrite H11 in H0.
+    rewrite H4, Znth_map in H12 by assumption. unfold flip in H12.
+    remember (Znth z roots) as root. rewrite <- H11 in H0. pose proof (Znth_In _ _ H0).
+    rewrite <- Heqroot in H13. rewrite H11 in H0. unfold Inhabitant_val in H12.
     assert (forall v, In (inr v) roots -> isptr (vertex_address g v)). {
-      intros. destruct H4. unfold vertex_address. rewrite Forall_forall in H14.
-      rewrite (filter_sum_right_In_iff v roots) in H13. apply H14 in H13.
-      destruct H13. apply graph_has_gen_start_isptr in H13.
+      intros. destruct H5. unfold vertex_address. rewrite Forall_forall in H15.
+      rewrite (filter_sum_right_In_iff v roots) in H14. apply H15 in H14.
+      destruct H14. apply graph_has_gen_start_isptr in H14.
       remember (gen_start g (vgeneration v)) as vv. destruct vv; try contradiction.
       simpl. exact I. }
     assert (is_pointer_or_integer (root2val g root)). {
       destruct root as [[? | ?] | ?]; simpl; auto.
       - destruct g0. simpl. exact I.
-      - specialize (H13 _ H12). apply isptr_is_pointer_or_integer. assumption. }
-    assert (0 <= Znth z (live_roots_indices f_info) < 1024) by
+      - specialize (H14 _ H13). apply isptr_is_pointer_or_integer. assumption. }
+    assert (0 <= Znth z (live_roots_indices f_info) < MAX_ARGS) by
         (apply (fi_index_range f_info), Znth_In; assumption).
-    forward; rewrite H11. 1: entailer!.
+    forward; rewrite H12. 1: entailer!.
     assert_PROP (valid_int_or_ptr (root2val g root)). {
-      gather_SEP 3 2. sep_apply (root_valid_int_or_ptr _ _ _ _ H12 H4). entailer!. }
+      gather_SEP 3 2. sep_apply (root_valid_int_or_ptr _ _ _ _ H13 H5). entailer!. }
     forward_call (root2val g root).
     remember (graph_rep g * heap_rest_rep (ti_heap t_info) * outlier_rep outlier)
-      as P. pose proof (graph_and_heap_rest_data_at_ _ _ _ H6 H).
-    unfold generation_data_at_ in H17. remember (gen_start g from) as fp.
+      as P. pose proof (graph_and_heap_rest_data_at_ _ _ _ H7 H).
+    unfold generation_data_at_ in H18. remember (gen_start g from) as fp.
     remember (nth_sh g from) as fsh. remember (gen_size t_info from) as gn.
     remember (WORD_SIZE * gn)%Z as fn.
     assert (P |-- (weak_derives P (memory_block fsh fn fp * TT) && emp) * P). {
-      apply weak_derives_strong. subst. sep_apply H17.
+      apply weak_derives_strong. subst. sep_apply H18.
       rewrite data_at__memory_block.
       rewrite sizeof_tarray_int_or_ptr; [Intros; cancel | unfold gen_size].
       destruct (total_space_tight_range (nth_space t_info from)). assumption. }
     destruct root as [[? | ?] | ?]; simpl root2val.
     + unfold odd_Z2val. apply semax_if_seq. forward_if.
-      1: exfalso; apply H19'; reflexivity.
+      1: exfalso; apply H20'; reflexivity.
       forward. Exists g t_info roots. rewrite <- Heqroot. entailer!.
       * simpl. split; [constructor | hnf; intuition].
       * unfold thread_info_rep. entailer!.
     + unfold GC_Pointer2val. destruct g0. apply semax_if_seq. forward_if.
-      2: exfalso; apply Int.one_not_zero in H19; assumption.
+      2: exfalso; apply Int.one_not_zero in H20; assumption.
       forward_call (Vptr b i). gather_SEP 3 6 2. rewrite <- sepcon_assoc.
-      rewrite <- HeqP. destruct H4.
+      rewrite <- HeqP. destruct H5.
       replace_SEP 0 ((weak_derives P (memory_block fsh fn fp * TT) && emp) * P) by
-          (entailer; assumption). clear H18. Intros. simpl root2val in *.
+          (entailer; assumption). clear H19. Intros. simpl root2val in *.
       assert (P |-- (weak_derives P (valid_pointer (Vptr b i) * TT) && emp) * P). {
         subst. cancel. apply andp_right. 2: cancel.
         assert (HS: emp |-- TT) by entailer; sep_apply HS; clear HS.
         apply derives_weak.
-        sep_apply (outlier_rep_valid_pointer roots outlier (GCPtr b i) H12 H4).
+        sep_apply (outlier_rep_valid_pointer roots outlier (GCPtr b i) H13 H5).
         simpl GC_Pointer2val. cancel. }
       replace_SEP 1 ((weak_derives P (valid_pointer (Vptr b i) * TT) && emp) * P) by
-          (entailer; assumption). Intros. clear H18.
+          (entailer; assumption). Intros. clear H19.
       forward_call (fsh, fp, fn, (Vptr b i), P). Intros v. destruct v.
-      * rewrite HeqP. Intros. gather_SEP 0 1. sep_apply H17. rewrite Heqfn in v.
-        sep_apply (outlier_rep_single_rep _ _ _ H12 H4). Intros. gather_SEP 0 2.
+      * rewrite HeqP. Intros. gather_SEP 0 1. sep_apply H18. rewrite Heqfn in v.
+        sep_apply (outlier_rep_single_rep _ _ _ H13 H5). Intros. gather_SEP 0 2.
         change (Vptr b i) with (GC_Pointer2val (GCPtr b i)) in v.
         pose proof (generation_share_writable (nth_gen g from)).
-        change (generation_sh (nth_gen g from)) with (nth_sh g from) in H18.
-        rewrite <- Heqfsh in H18. unfold generation_data_at_.
-        sep_apply (single_outlier_rep_memory_block_FF (GCPtr b i) fp gn fsh H18 v).
+        change (generation_sh (nth_gen g from)) with (nth_sh g from) in H19.
+        rewrite <- Heqfsh in H19. unfold generation_data_at_.
+        sep_apply (single_outlier_rep_memory_block_FF (GCPtr b i) fp gn fsh H19 v).
         assert_PROP False by entailer!. contradiction.
-      * apply semax_if_seq. forward_if. 1: exfalso; apply H18'; reflexivity.
+      * apply semax_if_seq. forward_if. 1: exfalso; apply H19'; reflexivity.
         forward. Exists g t_info roots. rewrite <- Heqroot. entailer!.
         -- split; [|split].
            ++ unfold roots_compatible. split; assumption.
            ++ simpl; constructor.
            ++ hnf; intuition.
         -- unfold thread_info_rep. entailer!.
-    + specialize (H13 _ H12). destruct (vertex_address g v) eqn:? ; try contradiction.
+    + specialize (H14 _ H13). destruct (vertex_address g v) eqn:? ; try contradiction.
       apply semax_if_seq. forward_if.
-      2: exfalso; apply Int.one_not_zero in H19; assumption.
-      clear H19 H19'. simpl in H14, H16. forward_call (Vptr b i).
+      2: exfalso; apply Int.one_not_zero in H20; assumption.
+      clear H20 H20'. simpl in H15, H17. forward_call (Vptr b i).
       rewrite <- Heqv0 in *. gather_SEP 3 6 2. rewrite <- sepcon_assoc, <- HeqP.
       replace_SEP 0 ((weak_derives P (memory_block fsh fn fp * TT) && emp) * P) by
-          (entailer; assumption). clear H18. Intros. assert (graph_has_v g v). {
-        destruct H4. rewrite Forall_forall in H18. apply H18.
+          (entailer; assumption). clear H19. Intros. assert (graph_has_v g v). {
+        destruct H5. rewrite Forall_forall in H19. apply H19.
         rewrite <- filter_sum_right_In_iff. assumption. }
       assert (P |-- (weak_derives P (valid_pointer (Vptr b i) * TT) && emp) * P). {
-        apply weak_derives_strong. subst. sep_apply (graph_rep_vertex_rep g v H18).
+        apply weak_derives_strong. subst. sep_apply (graph_rep_vertex_rep g v H19).
         Intros shh. unfold vertex_rep, vertex_at. remember (make_fields_vals g v).
         sep_apply (data_at_valid_ptr shh (tarray int_or_ptr_type (Zlength l)) l
                                      (vertex_address g v)).
@@ -169,26 +169,26 @@ Proof.
           rewrite Z.max_r; pose proof (raw_fields_range (vlabel g v)); omega.
         - rewrite Heqv0; cancel. }
       replace_SEP 1 (weak_derives P (valid_pointer (Vptr b i) * TT) && emp * P)
-        by (entailer; assumption). clear H19. Intros. rewrite <- Heqv0 in *.
+        by (entailer; assumption). clear H20. Intros. rewrite <- Heqv0 in *.
       forward_call (fsh, fp, fn, (vertex_address g v), P). Intros vv. rewrite HeqP.
-      sep_apply (graph_and_heap_rest_v_in_range_iff _ _ _ _ H H6 H18). Intros.
-      rewrite <- Heqfp, <- Heqgn, <- Heqfn in H19. destruct vv.
-      * Intros. rewrite H19 in v0. clear H19. apply semax_if_seq. forward_if.
-        2: exfalso; inversion H19. deadvars!. freeze [1; 2; 3; 4; 5; 6] FR.
-        clear H19 H19'. localize [vertex_rep (nth_sh g (vgeneration v)) g v].
+      sep_apply (graph_and_heap_rest_v_in_range_iff _ _ _ _ H H7 H19). Intros.
+      rewrite <- Heqfp, <- Heqgn, <- Heqfn in H20. destruct vv.
+      * Intros. rewrite H20 in v0. clear H20. apply semax_if_seq. forward_if.
+        2: exfalso; inversion H20. deadvars!. freeze [1; 2; 3; 4; 5; 6] FR.
+        clear H20 H20'. localize [vertex_rep (nth_sh g (vgeneration v)) g v].
         unfold vertex_rep, vertex_at. Intros. rewrite v0.
         assert (readable_share (nth_sh g from)) by
             (unfold nth_sh; apply writable_readable, generation_share_writable).
         sep_apply (data_at_minus1_address (nth_sh g from) (Z2val (make_header g v))
                                           (vertex_address g v)).
-        Intros. forward. clear H20. gather_SEP 0 1.
+        Intros. forward. clear H21. gather_SEP 0 1.
         replace_SEP 0 (vertex_rep (nth_sh g (vgeneration v)) g v) by
             (unfold vertex_rep, vertex_at; entailer!).
-        unlocalize [graph_rep g]. 1: apply (graph_vertex_ramif_stable _ _ H18).
-        apply semax_if_seq. forward_if; rewrite make_header_int_rep_mark_iff in H20.
+        unlocalize [graph_rep g]. 1: apply (graph_vertex_ramif_stable _ _ H19).
+        apply semax_if_seq. forward_if; rewrite make_header_int_rep_mark_iff in H21.
         -- deadvars!. localize [vertex_rep (nth_sh g (vgeneration v)) g v].
            rewrite v0. unfold vertex_rep, vertex_at. Intros.
-           unfold make_fields_vals at 2. rewrite H20.
+           unfold make_fields_vals at 2. rewrite H21.
            assert (0 <= 0 < Zlength (make_fields_vals g v)). {
              split. 1: omega. rewrite fields_eq_length.
              apply (proj1 (raw_fields_range (vlabel g v))). }
@@ -196,36 +196,36 @@ Proof.
                      (vertex_address g (copied_vertex (vlabel g v)))). {
              apply isptr_is_pointer_or_integer. unfold vertex_address.
              rewrite isptr_offset_val.
-             apply graph_has_gen_start_isptr, H8; assumption. }
+             apply graph_has_gen_start_isptr, H9; assumption. }
            forward. rewrite Znth_0_cons. gather_SEP 0 1.
            replace_SEP 0 (vertex_rep (nth_sh g (vgeneration v)) g v). {
              unfold vertex_rep, vertex_at. unfold make_fields_vals at 3.
-             rewrite H20. entailer!. }
-           unlocalize [graph_rep g]. 1: apply (graph_vertex_ramif_stable _ _ H18).
+             rewrite H21. entailer!. }
+           unlocalize [graph_rep g]. 1: apply (graph_vertex_ramif_stable _ _ H19).
            thaw FR. forward. forward. rewrite <- Heqroot.
-           rewrite if_true by reflexivity. rewrite H20.
+           rewrite if_true by reflexivity. rewrite H21.
            Exists g (upd_thread_info_arg
                        t_info
                        (Znth z (live_roots_indices f_info))
-                       (vertex_address g (copied_vertex (vlabel g v))) H15)
+                       (vertex_address g (copied_vertex (vlabel g v))) H16)
                   (upd_bunch z f_info roots (inr (copied_vertex (vlabel g v)))).
            unfold thread_info_rep. simpl. entailer!. split; split.
            ++ apply upd_fun_thread_arg_compatible. assumption.
-           ++ specialize (H8 _ H18 H20).
+           ++ specialize (H9 _ H19 H21).
               apply upd_roots_compatible; assumption.
            ++ apply fr_v_in_forwarded; [reflexivity | assumption].
            ++ hnf. intuition.
         -- forward. thaw FR. freeze [0; 1; 2; 3; 4; 5] FR.
-           rewrite make_header_Wosize by (apply not_true_is_false; assumption).
+           apply not_true_is_false in H21. rewrite make_header_Wosize by assumption.
            assert (0 <= Z.of_nat to < 12). {
-             clear -H H7. destruct H as [_ [_ ?]]. red in H7.
+             clear -H H8. destruct H as [_ [_ ?]]. red in H8.
              pose proof (spaces_size (ti_heap t_info)).
              rewrite Zlength_correct in H0. rep_omega. }
            assert (0 < Z.of_nat to) by omega. unfold heap_struct_rep.
-           destruct (gt_gs_compatible _ _ H _ H7) as [? [? ?]].
+           destruct (gt_gs_compatible _ _ H _ H8) as [? [? ?]].
            rewrite nth_space_Znth in *.
            remember (Znth (Z.of_nat to) (spaces (ti_heap t_info))) as sp_to.
-           assert (isptr (space_start sp_to)) by (rewrite <- H23; apply start_isptr).
+           assert (isptr (space_start sp_to)) by (rewrite <- H24; apply start_isptr).
            remember ((space_start (heap_head (ti_heap t_info)),
                       (Vundef,
                        offset_val
@@ -237,11 +237,11 @@ Proof.
              rewrite map_tl, Znth_tl by omega.
              replace (Z.of_nat to - 1 + 1) with (Z.of_nat to) by omega.
              rewrite Znth_map by (rewrite spaces_size; rep_omega). reflexivity. }
-           unfold Inhabitant_pair, Inhabitant_val, Inhabitant in H27.
-           forward; rewrite H27; unfold space_tri. 1: entailer!.
+           unfold Inhabitant_pair, Inhabitant_val, Inhabitant in H28.
+           forward; rewrite H28; unfold space_tri. 1: entailer!.
            forward. simpl sem_binary_operation'.
            rewrite sapi_ptr_val by assumption. Opaque Znth. forward. Transparent Znth.
-           rewrite sapi_ptr_val by assumption. rewrite H27. unfold space_tri.
+           rewrite sapi_ptr_val by assumption. rewrite H28. unfold space_tri.
            rewrite <- Z.add_assoc.
            replace (1 + Zlength (raw_fields (vlabel g v))) with (vertex_size g v) by
                (unfold vertex_size; omega). thaw FR. freeze [0; 2; 3; 4; 5; 6] FR.
@@ -251,7 +251,7 @@ Proof.
                                  (vertex_size g v)). {
              red. split. 1: pose proof (svs_gt_one g v); omega.
              transitivity (unmarked_gen_size g (vgeneration v)).
-             - apply single_unmarked_le; [|apply not_true_is_false]; assumption.
+             - apply single_unmarked_le; assumption.
              - red in H1. unfold rest_gen_size in H1. subst from.
                rewrite nth_space_Znth in H1. assumption. }
            assert (Hn: space_start (Znth (Z.of_nat to) (spaces (ti_heap t_info))) <>
@@ -273,11 +273,11 @@ Proof.
                apply (heap_spaces_nil (ti_heap t_info)). rewrite Hs. reflexivity. }
              replace (Z.of_nat to - 1 + 1) with (Z.of_nat to) by omega.
              unfold cut_thread_info, heap_struct_rep. simpl ti_heap_p. entailer!. }
-           sep_apply (graph_vertex_ramif_stable _ _ H18). Intros.
+           sep_apply (graph_vertex_ramif_stable _ _ H19). Intros.
            freeze [1; 2; 3; 4; 5] FR. deadvars!. rewrite v0.
            remember (nth_sh g from) as shv.
            assert (writable_share (space_sh sp_to)) by
-               (rewrite <- H24; apply generation_share_writable).
+               (rewrite <- H25; apply generation_share_writable).
            remember (space_sh sp_to) as sht.
            rewrite (data_at__tarray_value _ _ 1). 2: unfold vertex_size; rep_omega.
            Intros.
@@ -294,7 +294,7 @@ Proof.
              rewrite if_true by assumption. simpl. rewrite offset_offset_val.
              f_equal. omega. }
            forward. sep_apply (field_at_data_at_cancel
-                                 sht tuint (Z2val (make_header g v)) v1). clear H29.
+                                 sht tuint (Z2val (make_header g v)) v1). clear H30.
            subst v1. rewrite offset_offset_val.
            replace (vertex_size g v - 1) with (Zlength (raw_fields (vlabel g v)))
              by (unfold vertex_size; omega).
@@ -305,13 +305,18 @@ Proof.
            thaw FR. freeze [0; 1; 2; 3; 4; 5] FR. rename i into j. deadvars!.
            remember (Zlength (raw_fields (vlabel g v))) as n.
            assert (isptr nv) by (subst nv; rewrite isptr_offset_val; assumption).
+           remember (field_address thread_info_type
+                                   [ArraySubsc (Znth z (live_roots_indices f_info));
+                                    StructField _args] ti) as p_addr.
            forward_for_simple_bound
              n
              (EX i: Z,
               PROP ( )
               LOCAL (temp _new nv;
                      temp _sz (vint n);
-                     temp _v (vertex_address g v))
+                     temp _v (vertex_address g v);
+                     temp _p p_addr;
+                     temp _depth (vint depth))
               SEP (vertex_rep shv g v;
                    data_at sht (tarray int_or_ptr_type i)
                            (sublist 0 i (make_fields_vals g v)) nv;
@@ -327,8 +332,8 @@ Proof.
                 [|reflexivity | assumption | reflexivity]. entailer!.
            ++ unfold vertex_rep, vertex_at. Intros.
               rewrite fields_eq_length, <- Heqn. forward.
-              ** entailer!. pose proof (mfv_all_is_ptr_or_int _ _ H8 H9 H18).
-                 rewrite Forall_forall in H41. apply H41, Znth_In.
+              ** entailer!. pose proof (mfv_all_is_ptr_or_int _ _ H9 H10 H19).
+                 rewrite Forall_forall in H42. apply H42, Znth_In.
                  rewrite fields_eq_length. assumption.
               ** rewrite (data_at__tarray_value _ _ 1) by omega. Intros.
                  rewrite data_at__singleton_array_eq.
@@ -362,21 +367,21 @@ Proof.
                 apply data_at__value_0_size. }
               assert (nv = vertex_address g (new_copied_v g to)). {
                 subst nv. unfold vertex_address. unfold new_copied_v. simpl. f_equal.
-                - unfold vertex_offset. simpl. rewrite H25. reflexivity.
+                - unfold vertex_offset. simpl. rewrite H26. reflexivity.
                 - unfold gen_start. rewrite if_true by assumption.
-                  rewrite H23. reflexivity. }
+                  rewrite H24. reflexivity. }
               gather_SEP 1 2 3.
               replace_SEP
                 0 (vertex_at (nth_sh g to)
                              (vertex_address g (new_copied_v g to))
                              (make_header g v) (make_fields_vals g v)). {
-                normalize. rewrite <- H24.
+                normalize. rewrite <- H25.
                 change (generation_sh (nth_gen g to)) with (nth_sh g to).
                 rewrite <- fields_eq_length in Heqn.
                 replace (offset_val (WORD_SIZE * used_space sp_to) (space_start sp_to))
                   with (offset_val (- WORD_SIZE) nv) by
                     (rewrite Heqnv; rewrite offset_offset_val; f_equal; rep_omega).
-                rewrite <- H30. unfold vertex_at; entailer!. }
+                rewrite <- H31. unfold vertex_at; entailer!. }
               gather_SEP 0 1. rewrite (copied_v_derives_new_g g v to) by assumption.
               freeze [1; 2; 3; 4] FR. remember (lgraph_add_copied_v g v to) as g'.
               assert (vertex_address g' v = vertex_address g v) by
@@ -384,24 +389,25 @@ Proof.
               assert (vertex_address g' (new_copied_v g to) =
                       vertex_address g (new_copied_v g to)) by
                   (subst g'; apply lacv_vertex_address_new; assumption).
-              rewrite <- H31. rewrite <- H32 in H30.
+              rewrite <- H32. rewrite <- H33 in H31.
               assert (writable_share (nth_sh g' (vgeneration v))) by
                   (unfold nth_sh; apply generation_share_writable).
               assert (graph_has_v g' (new_copied_v g to)) by
                   (subst g'; apply lacv_graph_has_v_new; assumption).
-              sep_apply (graph_rep_valid_int_or_ptr _ _ H34). Intros.
-              rewrite <- H30 in H35. assert (graph_has_v g' v) by
+              sep_apply (graph_rep_valid_int_or_ptr _ _ H35). Intros.
+              rewrite <- H31 in H36. assert (graph_has_v g' v) by
                   (subst g'; apply lacv_graph_has_v_old; assumption).
-              sep_apply (graph_vertex_lmc_ramif g' v (new_copied_v g to) H36).
-              Intros. freeze [1; 2] FR1. unfold vertex_rep, vertex_at. Intros.
+              remember (nth_sh g' (vgeneration v)) as sh'.
+              sep_apply (graph_vertex_lmc_ramif g' v (new_copied_v g to) H37).
+              rewrite <- Heqsh'. Intros. freeze [1; 2] FR1.
+              unfold vertex_rep, vertex_at. Intros.
               sep_apply (data_at_minus1_address
-                           (nth_sh g' (vgeneration v)) (Z2val (make_header g' v))
-                           (vertex_address g' v)). Intros. forward. clear H36.
+                           sh' (Z2val (make_header g' v)) (vertex_address g' v)).
+              Intros. forward. clear H38.
               sep_apply (field_at_data_at_cancel
-                           (nth_sh g' (vgeneration v)) tuint (vint 0)
+                           sh' tuint (vint 0)
                            (offset_val (- WORD_SIZE) (vertex_address g' v))).
-              forward_call (nv). remember (nth_sh g' (vgeneration v)) as sh'.
-              remember (make_fields_vals g' v) as l'.
+              forward_call (nv). remember (make_fields_vals g' v) as l'.
               assert (0 < Zlength l'). {
                 subst l'. rewrite fields_eq_length.
                 apply (proj1 (raw_fields_range (vlabel g' v))). }
@@ -411,19 +417,45 @@ Proof.
                            field_address int_or_ptr_type [] (vertex_address g' v)). {
                 clear. entailer!. unfold field_address. rewrite if_true by assumption.
                 simpl. rewrite isptr_offset_val_zero. 1: reflexivity.
-                destruct H3. assumption. } forward. clear H37.
+                destruct H3. assumption. } forward. clear H39.
               sep_apply (field_at_data_at_cancel
                            sh' int_or_ptr_type nv (vertex_address g' v)).
-              gather_SEP 1 0 3. rewrite H30. subst l'.
-              rewrite <- sepcon_assoc, <- lmc_vertex_rep_eq. subst sh'.
+              gather_SEP 1 0 3. rewrite H31. subst l'.
+              rewrite <- sepcon_assoc, <- lmc_vertex_rep_eq.
               thaw FR1. gather_SEP 0 1.
-              sep_apply (wand_frame_elim
-                           (vertex_rep (nth_sh g' (vgeneration v))
-                                       (lgraph_mark_copied g' v (new_copied_v g to)) v)
-                           (graph_rep (lgraph_mark_copied g' v (new_copied_v g to)))).
-              admit.
-      * apply semax_if_seq. forward_if. 1: exfalso; apply H20'; reflexivity.
-        rewrite H19 in n. forward. rewrite <- Heqroot. rewrite if_false by assumption.
+              sep_apply
+                (wand_frame_elim
+                   (vertex_rep sh' (lgraph_mark_copied g' v (new_copied_v g to)) v)
+                   (graph_rep (lgraph_mark_copied g' v (new_copied_v g to)))).
+              rewrite <- (lmc_vertex_address g' v (new_copied_v g to)) in *. subst g'.
+              change (lgraph_mark_copied
+                        (lgraph_add_copied_v g v to) v (new_copied_v g to))
+                with (lgraph_copy_v g v to) in *.
+              remember (lgraph_copy_v g v to) as g'. rewrite <- H31 in *. thaw FR.
+              forward_call (nv). subst p_addr.
+              remember (cut_thread_info t_info (Z.of_nat to) (vertex_size g v) Hi Hh)
+                as t_info'. unfold thread_info_rep. Intros. forward.
+              remember (Znth z (live_roots_indices f_info)) as lz. gather_SEP 1 2 3.
+              replace_SEP 0 (thread_info_rep
+                               sh (update_thread_info_arg t_info' lz nv H16) ti). {
+                unfold thread_info_rep. simpl heap_head. simpl ti_heap_p.
+                simpl ti_args. simpl ti_heap. clear Heqt_info'. entailer!. }
+              remember (update_thread_info_arg t_info' lz nv H16) as t. subst t_info'.
+              rename t into t_info'. apply semax_if_seq. forward_if.
+              ** admit.
+              ** assert (Z.to_nat depth = O) by
+                    (assert (depth = 0) by omega; rewrite H40; reflexivity).
+                deadvars!. clear Heqnv H33. forward.
+                 rewrite <- Heqroot. rewrite if_true by reflexivity. rewrite H21.
+                 remember (Znth z (live_roots_indices f_info)) as lz.
+                 remember (vertex_address (lgraph_copy_v g v to) (new_copied_v g to))
+                   as nv. remember (cut_thread_info
+                                      t_info (Z.of_nat to) (vertex_size g v) Hi Hh).
+                 Exists (lgraph_copy_v g v to) (update_thread_info_arg t lz nv H16)
+                        (upd_bunch z f_info roots (inr (new_copied_v g to))).
+                 entailer!. rewrite H40. admit.
+      * apply semax_if_seq. forward_if. 1: exfalso; apply H21'; reflexivity.
+        rewrite H20 in n. forward. rewrite <- Heqroot. rewrite if_false by assumption.
         Exists g t_info roots. simpl. entailer!.
         -- split; [constructor; assumption | hnf; intuition].
         -- unfold thread_info_rep. entailer!.
